major refactoring

Isabelle/IMAP.thy
@@ -13,7 +13,6 @@ begin
 -- "Type definition: 'a is the set of all folder names, 'b is the set of all message names"
 type_synonym ('a, 'b) imap = "'a orset \<times> ('a \<rightharpoonup> 'b set)"
 
-
 abbreviation folderset ::
   "('a, 'b) imap \<Rightarrow> 'a orset"
 where
@@ -31,12 +30,10 @@ where
   "validState I = ((\<forall> (a, _) \<in> folderset I . (filesystem I) a \<noteq> None)
   \<and> (\<forall> f . (filesystem I) f \<noteq> None \<longrightarrow> (\<exists> (a, _) \<in> folderset I . a = f)))"
 
-
-definition replaceMsg ::
+definition Msg ::
   "'b \<Rightarrow> 'b \<Rightarrow> 'b set \<Rightarrow> 'b set"
 where
-  "replaceMsg msgold msgnew S = (S - {msgold}) \<union> {msgnew}"
-
+  "Msg msgold msgnew S = (S - {msgold}) \<union> {msgnew}"
 
 definition msgLookup ::
   "'a \<Rightarrow> 'b \<Rightarrow> ('a, 'b) imap \<Rightarrow> bool"
@@ -47,50 +44,39 @@ where
       Some msgset \<Rightarrow> msg \<in> msgset
   )"
 
-
-
 -- "#######################"
 -- "### IMAP Operations ###"
 -- "#######################"
 
-
-definition CREATE_atSource ::
-  "'a \<Rightarrow> ('a, 'b) imap \<Rightarrow> bool"
+definition create_pre ::
+  "'a \<Rightarrow> nat \<Rightarrow> ('a, 'b) imap \<Rightarrow> bool"
 where
-  "CREATE_atSource f I = (\<nexists> n . (f, n) \<in> folderset I)"
+  "create_pre f n I = (add_pre n (folderset I) \<and> \<not> lookup f (folderset I))"
 
-definition CREATE_downstream ::
+definition create ::
   "'a \<Rightarrow> nat \<Rightarrow> ('a, 'b) imap \<Rightarrow> ('a, 'b) imap"
 where
-  "CREATE_downstream f n I = (add f n (folderset I), (filesystem I)(f := Some {}))"
+  "create f n I = (add f n (folderset I), (filesystem I)(f := Some {}))"
 
-
-definition DELETE_atSource ::
-  "'a \<Rightarrow> ('a, 'b) imap \<Rightarrow> 'a orset"
+definition delete_pre ::
+  "'a \<Rightarrow> 'a orset \<Rightarrow> ('a, 'b) imap \<Rightarrow> bool"
 where
-  "DELETE_atSource e I = remove_atSource e (folderset I)"
+  "delete_pre f R I = remove_pre f R (folderset I)"
 
--- "unused"
-definition DELETE_atSource_pre ::
-  "'a \<Rightarrow> ('a, 'b) imap \<Rightarrow> bool"
-where
-  "DELETE_atSource_pre e I = (\<exists> (a, _) \<in> folderset I . a = e)"
-
-definition DELETE_downstream ::
+definition delete ::
   "'a \<Rightarrow> 'a orset \<Rightarrow> ('a, 'b) imap \<Rightarrow> ('a, 'b) imap"
 where
-  "DELETE_downstream e R I = (remove_downstream R (folderset I), (filesystem I)(e := None))"
+  "delete f R I = (remove R (folderset I), (filesystem I)(f := None))"
 
-
-definition APPEND_atSource ::
+definition append_pre ::
   "'a \<Rightarrow> 'b \<Rightarrow> ('a, 'b) imap \<Rightarrow> bool"
 where
-  "APPEND_atSource f m I = (\<exists> (a, _) \<in> folderset I . a = f \<and> \<not> msgLookup f m I)"
+  "append_pre f m I = (\<exists> (a, _) \<in> folderset I . a = f \<and> \<not> msgLookup f m I)"
 
-definition APPEND_downstream ::
+definition append ::
   "'a \<Rightarrow> 'b \<Rightarrow> ('a, 'b) imap \<Rightarrow> ('a, 'b) imap"
 where
-  "APPEND_downstream f m I =
+  "append f m I =
   (folderset I,
   (case (filesystem I)(f) of
       None \<Rightarrow> filesystem I |
@@ -98,21 +84,20 @@ where
   ))"
 
 
-definition STORE_atSource ::
+definition store_pre ::
   "'a \<Rightarrow> 'b \<Rightarrow> 'b \<Rightarrow> ('a, 'b) imap \<Rightarrow> bool"
 where
-  "STORE_atSource f msgold msgnew I = ((\<exists> (a, _) \<in> folderset I . a = f) \<and> msgLookup f msgold I \<and> \<not>(msgLookup f msgnew I))"
+  "store_pre f msgold msgnew I = ((\<exists> (a, _) \<in> folderset I . a = f) \<and> msgLookup f msgold I \<and> \<not>(msgLookup f msgnew I))"
 
-definition STORE_downstream ::
+definition store ::
   "'a \<Rightarrow> 'b \<Rightarrow> 'b \<Rightarrow> ('a, 'b) imap \<Rightarrow> ('a, 'b) imap"
 where
-  "STORE_downstream f msgold msgnew I =
+  "store f msgold msgnew I =
   (folderset I,
   (case (filesystem I)(f) of
       None \<Rightarrow> filesystem I |
-      Some msgset \<Rightarrow> (filesystem I)(f := Some (replaceMsg msgold msgnew msgset))
+      Some msgset \<Rightarrow> (filesystem I)(f := Some (Msg msgold msgnew msgset))
   ))"
-
 
 definition EXPUNGE_atSource ::
   "'a \<Rightarrow> 'b \<Rightarrow> ('a, 'b) imap \<Rightarrow> bool"
@@ -142,34 +127,32 @@ fixes
   f1 :: "'a" and
   m1 :: "'b"
 assumes
-  O1pre: " APPEND_atSource f1 m1 I" and
+  O1pre: " append_pre f1 m1 I" and
   validS: "validState I"
-shows "filesystem (APPEND_downstream f1 m1 I) f1 \<noteq> None"
+shows "filesystem (append f1 m1 I) f1 \<noteq> None"
 proof -
   have "filesystem I f1 \<noteq> None"
   using O1pre validS
-  unfolding validState_def APPEND_atSource_def
+  unfolding validState_def append_pre_def
   by auto
 
   thus ?thesis
   using validS O1pre
-  unfolding APPEND_downstream_def validState_def APPEND_atSource_def
+  unfolding append_def validState_def append_pre_def
   by auto
 qed
-
 
 lemma append_folderset:
 fixes
   I :: "('a, 'b) imap" and
   f :: "'a" and
   m :: "'b"
-shows "folderset (APPEND_downstream f m I) = folderset I"
+shows "folderset (append f m I) = folderset I"
 proof -
   show ?thesis
-  unfolding APPEND_downstream_def
+  unfolding append_def
   by auto
 qed
-
 
 lemma append_filesystem:
 fixes
@@ -177,12 +160,12 @@ fixes
   f1 :: "'a" and
   m1 :: "'b"
 assumes
-  O1pre: " APPEND_atSource f1 m1 I" and
+  O1pre: " append_pre f1 m1 I" and
   validS: "validState I"
-shows "\<forall> f . f \<noteq> f1 \<longrightarrow> filesystem (APPEND_downstream f1 m1 I) f = filesystem I f"
+shows "\<forall> f . f \<noteq> f1 \<longrightarrow> filesystem (append f1 m1 I) f = filesystem I f"
 proof -
   show ?thesis
-  by (simp add: APPEND_downstream_def option.case_eq_if)
+  by (simp add: append_def option.case_eq_if)
 qed
 
 
@@ -190,10 +173,10 @@ lemma store_folderset:
 fixes
   I :: "('a, 'b) imap" and
   f :: "'a"
-shows "folderset (STORE_downstream f msgold msgnew I) = folderset I"
+shows "folderset (store f msgold msgnew I) = folderset I"
 proof -
   show ?thesis
-  unfolding STORE_downstream_def
+  unfolding store_def
   by auto
 qed
 
@@ -202,10 +185,10 @@ lemma store_filesystem:
 fixes
   I :: "('a, 'b) imap" and
   f1 :: "'a"
-shows "\<forall> f. f \<noteq> f1 \<longrightarrow> filesystem (STORE_downstream f1 msgold msgnew I) f = filesystem I f"
+shows "\<forall> f. f \<noteq> f1 \<longrightarrow> filesystem (store f1 msgold msgnew I) f = filesystem I f"
 proof -
   show ?thesis
-  unfolding STORE_downstream_def
+  unfolding store_def
   by (simp add: option.case_eq_if)
 qed
 
@@ -217,11 +200,11 @@ fixes
   msgold :: "'b" and
   msgnew :: "'b"
 assumes
-  pre: "STORE_atSource f1 msgold msgnew I"
-shows "filesystem (STORE_downstream f1 msgold msgnew I) f1 \<noteq> None"
+  pre: "store_pre f1 msgold msgnew I"
+shows "filesystem (store f1 msgold msgnew I) f1 \<noteq> None"
 proof -
   show ?thesis
-  using pre unfolding STORE_downstream_def STORE_atSource_def msgLookup_def
+  using pre unfolding store_def store_pre_def msgLookup_def
   by (metis fun_upd_same option.case_eq_if option.simps(3) snd_conv)
 qed
 
@@ -239,11 +222,11 @@ fixes
   n :: nat
 assumes
   validS: "validState I"
-shows "validState (CREATE_downstream e n I)"
+shows "validState (create e n I)"
 proof -
   show ?thesis
   using validS
-  unfolding CREATE_downstream_def add_def validState_def CREATE_atSource_def
+  unfolding create_def add_def validState_def create_pre_def
   apply simp
   by (simp add: split_def)
 qed
@@ -255,27 +238,27 @@ fixes
   R :: "'a orset" and
   e1 :: "'a"
 assumes
-  O1pre: "R = DELETE_atSource e1 I" and
+  O1pre: "delete_pre e1 R I" and
   validS: "validState I"
-shows "validState (DELETE_downstream e1 R I)"
+shows "validState (delete e1 R I)"
 proof -
-  have A1: "\<forall> (a, b) \<in> folderset I. a \<noteq> e1 \<longrightarrow> (a, b) \<in> folderset (DELETE_downstream e1 R I)"
+  have A1: "\<forall> (a, b) \<in> folderset I. a \<noteq> e1 \<longrightarrow> (a, b) \<in> folderset (delete e1 R I)"
   using O1pre
-  unfolding DELETE_downstream_def remove_downstream_def DELETE_atSource_def remove_atSource_def
+  unfolding delete_def remove_def delete_pre_def remove_pre_def
   by auto
 
-  have "\<forall> (a, _) \<in> folderset (DELETE_downstream e1 R I). a \<noteq> e1"
+  have "\<forall> (a, _) \<in> folderset (delete e1 R I). a \<noteq> e1"
   using O1pre
-  unfolding DELETE_downstream_def remove_downstream_def DELETE_atSource_def remove_atSource_def
+  unfolding delete_def remove_def delete_pre_def remove_pre_def
   by auto
 
-  hence "(\<forall> (a, _) \<in> folderset (DELETE_downstream e1 R I) . (filesystem (DELETE_downstream e1 R I)) a \<noteq> None)" using validS
-  unfolding validState_def DELETE_downstream_def remove_downstream_def DELETE_atSource_def remove_atSource_def
+  hence "(\<forall> (a, _) \<in> folderset (delete e1 R I) . (filesystem (delete e1 R I)) a \<noteq> None)" using validS
+  unfolding validState_def delete_def remove_def delete_pre_def remove_pre_def
   by fastforce
 
   thus ?thesis
   using validS A1
-  unfolding validState_def DELETE_atSource_def DELETE_downstream_def remove_atSource_def remove_downstream_def
+  unfolding validState_def delete_pre_def delete_def remove_def remove_pre_def
   apply simp
   by blast
 qed
@@ -287,21 +270,21 @@ fixes
   f1 :: "'a" and
   m1 :: "'b"
 assumes
-  O1pre: " APPEND_atSource f1 m1 I" and
+  O1pre: " append_pre f1 m1 I" and
   validS: "validState I"
-shows "validState (APPEND_downstream f1 m1 I)"
+shows "validState (append f1 m1 I)"
 proof -
-  have "folderset (APPEND_downstream f1 m1 I) = folderset I"
-  unfolding APPEND_downstream_def
+  have "folderset (append f1 m1 I) = folderset I"
+  unfolding append_def
   by auto
 
-  hence "(\<forall>f. filesystem (APPEND_downstream f1 m1 I) f \<noteq> None \<longrightarrow> (\<exists> (a, _) \<in>folderset (APPEND_downstream f1 m1 I). a = f))"
+  hence "(\<forall>f. filesystem (append f1 m1 I) f \<noteq> None \<longrightarrow> (\<exists> (a, _) \<in>folderset (append f1 m1 I). a = f))"
   using O1pre
-  by (metis (no_types, lifting) APPEND_atSource_def append_filesystem case_prod_beta' validS validState_def)
+  by (metis (no_types, lifting) append_pre_def append_filesystem case_prod_beta' validS validState_def)
 
   thus ?thesis
   using O1pre validS
-  unfolding validState_def APPEND_downstream_def
+  unfolding validState_def append_def
   apply simp
   by (smt case_prodE fun_upd_apply old.prod.case option.case_eq_if)
 qed
@@ -314,13 +297,13 @@ fixes
   msgold :: "'b" and
   msgnew :: "'b"
 assumes
-  O1pre : "STORE_atSource f msgold msgnew I" and
+  O1pre : "store_pre f msgold msgnew I" and
   validS: "validState I"
-shows "validState (STORE_downstream f msgold msgnew I)"
+shows "validState (store f msgold msgnew I)"
 proof -
   show ?thesis
   using O1pre validS
-  unfolding STORE_downstream_def STORE_atSource_def msgLookup_def replaceMsg_def
+  unfolding store_def store_pre_def msgLookup_def Msg_def
   by (simp add: case_prod_beta' fun_upd_same option.case_eq_if validState_def)
 qed
 
@@ -360,83 +343,137 @@ qed
 
 
 -- "Case 1"
-lemma commCREATE_CREATE:
+lemma comm_create_create:
 fixes
   I :: "('a, 'b) imap" and
-  e1 :: "'a" and
-  e2 :: "'a" and
+  f1 :: "'a" and
+  f2 :: "'a" and
   n1 :: nat and
   n2 :: nat
 assumes
-  n1neqn2: "n1 \<noteq> n2"
-shows "CREATE_downstream e1 n1 (CREATE_downstream e2 n2 I) = CREATE_downstream e2 n2 (CREATE_downstream e1 n1 I)"
+  O1pre: "create_pre f1 n1 I " and
+  O2pre: "create_pre f2 n2 I" 
+shows "create f1 n1 (create f2 n2 I) = create f2 n2 (create f1 n1 I)"
 proof -
-  show ?thesis
-  unfolding CREATE_downstream_def
-  using commAdd n1neqn2
-  by fastforce
+  show ?thesis 
+    using orset_comm[of "Add f1 n1" "folderset I" "Add f2 n2"] O1pre O2pre
+    unfolding create_pre_def create_def 
+    by auto
 qed
 
-
 -- "Case 2"
-lemma commCREATE_DELETE:
+lemma comm_create_delete:
+fixes
+  I :: "('a, 'b) imap" and
+  R :: "'a orset" and
+  f1 :: "'a" and
+  f2 :: "'a" and
+  n :: nat
+assumes
+  O1pre: "delete_pre f1 R I " and
+  O2pre: "create_pre f2 n I" 
+shows "delete f1 R (create f2 n I) = create f2 n (delete f1 R I)"
+proof -
+  have A1: "folderset (delete f1 R (create f2 n I)) = folderset (create f2 n (delete f1 R I))"
+    using O1pre O2pre orset_comm[of "Remove f1 R" "folderset I" "Add f2 n"]
+    by (simp add: delete_pre_def create_pre_def delete_def create_def)
+  have "filesystem (delete f1 R (create f2 n I)) = filesystem (create f2 n (delete f1 R I))"
+    using O1pre O2pre
+    unfolding delete_def create_def delete_pre_def remove_pre_def create_pre_def     
+    by fastforce
+  thus ?thesis using A1 by (simp add: delete_def)
+qed
+
+-- "Case 6"
+lemma comm_delete_delete:
 fixes
   I :: "('a, 'b) imap" and
   R1 :: "'a orset" and
-  e1 :: "'a" and
-  e2 :: "'a" and
-  n :: nat
+  R2 :: "'a orset" and
+  f1 :: "'a" and
+  f2 :: "'a"
 assumes
-  O1R1: " R1 = DELETE_atSource e1 I" and
-  freshn: "fresh n (folderset I)" and
-  O2pre: "CREATE_atSource e2 I" and
-  lookupe1: "lookup e1 (folderset I)"
-shows "DELETE_downstream e1 R1 (CREATE_downstream e2 n I) = CREATE_downstream e2 n (DELETE_downstream e1 R1 I)"
+  O1pre: "delete_pre f1 R1 I" and
+  O2pre: "delete_pre f2 R2 I"
+shows "delete f2 R2 (delete f1 R1 I) = delete f1 R1 (delete f2 R2 I)"
 proof -
-  have fset: "folderset (DELETE_downstream e1 R1 (CREATE_downstream e2 n I)) = folderset (CREATE_downstream e2 n (DELETE_downstream e1 R1 I))"
-  using O1R1 freshn
-  unfolding DELETE_downstream_def CREATE_downstream_def fresh_def commAddRemove DELETE_atSource_def remove_atSource_def remove_downstream_def add_def
-  by auto
-
-  have "filesystem (DELETE_downstream e1 R1 (CREATE_downstream e2 n I)) = filesystem (CREATE_downstream e2 n (DELETE_downstream e1 R1 I))"
-  using O1R1 O2pre lookupe1
-  unfolding DELETE_downstream_def CREATE_downstream_def DELETE_atSource_def remove_atSource_def CREATE_atSource_def validState_def lookup_def
-  by fastforce
-
-  thus ?thesis
-  using fset
-  unfolding DELETE_downstream_def
-  by auto
+  have A1: "folderset(delete f2 R2 (delete f1 R1 I)) = folderset(delete f1 R1 (delete f2 R2 I))"
+    using O1pre O2pre orset_comm[of "Remove f1 R1" "folderset I" "Remove f2 R2"]
+    by (simp add: delete_pre_def delete_def)
+  have "filesystem(delete f2 R2 (delete f1 R1 I)) = filesystem(delete f1 R1 (delete f2 R2 I))"
+    using O1pre O2pre
+    by (metis (mono_tags, lifting) delete_def fun_upd_twist snd_conv)    
+  thus ?thesis using A1 by (simp add: delete_def)
 qed
-
-
+  
 -- "Case 3"
-lemma commCREATE_APPEND:
+-- "TODO: remove smt"
+lemma comm_create_append:
 fixes
   I :: "('a, 'b) imap" and
-  e :: "'a" and
+  f1 :: "'a" and
   n :: nat and
-  f :: "'a" and
+  f2 :: "'a" and
   m :: "'b"
 assumes
-  O1pre: " APPEND_atSource f m I" and
-  O2pre: " CREATE_atSource e I"
-shows "APPEND_downstream f m (CREATE_downstream e n I) = CREATE_downstream e n (APPEND_downstream f m I)"
+  O1pre: "append_pre f1 m I" and
+  O2pre: "create_pre f2 n I"
+shows "append f1 m (create f2 n I) = create f2 n (append f1 m I)"
 proof -
-  have "filesystem(APPEND_downstream f m (CREATE_downstream e n I)) = filesystem(CREATE_downstream e n (APPEND_downstream f m I))"
-  using O1pre O2pre
-  unfolding APPEND_atSource_def APPEND_downstream_def CREATE_atSource_def CREATE_downstream_def
-  by (smt case_prodE fun_upd_apply fun_upd_twist option.case_eq_if prod.sel(2))
-
-  thus ?thesis
-  using append_folderset[of f m I]
-  unfolding APPEND_downstream_def CREATE_downstream_def
-  by auto
+  have "filesystem(append f1 m (create f2 n I)) = filesystem(create f2 n (append f1 m I))"
+    using O1pre O2pre
+    unfolding append_pre_def append_def create_pre_def create_def lookup_def apply simp
+    by (smt case_prodE eq_snd_iff fun_upd_twist option.case_eq_if)
+  thus ?thesis by (simp add: append_def create_def)
 qed
-
-
+  
+-- "Case 7"
+lemma comm_delete_append:
+fixes
+  I :: "('a, 'b) imap" and
+  f1 :: "'a" and
+  f2 :: "'a" and
+  m :: "'b" and
+  R :: "'a orset"
+assumes
+  O1pre: "append_pre f1 m I" and
+  O2pre: "delete_pre f2 R I"
+shows "append f1 m (delete f2 R I) = delete f2 R (append f1 m I)"
+proof -
+  have A1: "folderset(append f1 m (delete f2 R I)) = folderset(delete f2 R (append f1 m I))"
+    by (simp add: append_folderset delete_def)
+  have "filesystem(append f1 m (delete f2 R I)) = filesystem(delete f2 R (append f1 m I))"
+    using O1pre O2pre
+    unfolding append_pre_def append_def delete_pre_def delete_def
+    by (simp add: fun_upd_twist option.case_eq_if)
+  thus ?thesis using A1 prod_eqI  by blast
+qed
+  
+-- "Case 10"
+-- "TODO: remove smt"
+lemma comm_append_append:
+fixes
+  I :: "('a, 'b) imap" and
+  f1 :: "'a" and
+  f2 :: "'a" and
+  m1 :: "'b" and
+  m2 :: "'b"
+assumes
+  O1pre: "append_pre f1 m1 I" and
+  O2pre: "append_pre f2 m2 I"
+shows "append f1 m1 (append f2 m2 I) = append f2 m2 (append f1 m1 I)"
+proof -
+  have A1: "folderset(append f1 m1 (append f2 m2 I)) = folderset(append f2 m2 (append f1 m1 I))"
+    by (simp add: append_def)
+  have "filesystem(append f1 m1 (append f2 m2 I)) = filesystem(append f2 m2 (append f1 m1 I))"
+    using O1pre O2pre
+    unfolding append_def append_pre_def msgLookup_def
+    by (smt Un_insert_right fun_upd_twist fun_upd_upd insert_commute map_upd_Some_unfold option.case_eq_if option.collapse option.simps(3) snd_conv sup_bot.right_neutral)
+  thus ?thesis using A1 by (simp add: prod_eq_iff)
+qed
+  
 -- "Case 4"
-lemma commCREATE_STORE:
+lemma comm_create_store:
 fixes
   I :: "('a, 'b) imap" and
   f1 :: "'a" and
@@ -445,23 +482,251 @@ fixes
   mn :: "'b" and
   n :: nat
 assumes
-  O1pre: " STORE_atSource f1 mo mn I" and
-  O2pre: " CREATE_atSource f2 I"
-shows "STORE_downstream f1 mo mn (CREATE_downstream f2 n I) = CREATE_downstream f2 n (STORE_downstream f1 mo mn I)"
+  O1pre: "store_pre f1 mo mn I" and
+  O2pre: "create_pre f2 n I"
+shows "store f1 mo mn (create f2 n I) = create f2 n (store f1 mo mn I)"
 proof -
-  have A1: "folderset (STORE_downstream f1 mo mn (CREATE_downstream f2 n I)) = folderset (CREATE_downstream f2 n (STORE_downstream f1 mo mn I))"
-  by (simp add: CREATE_downstream_def store_folderset)
-
-  have "filesystem (STORE_downstream f1 mo mn (CREATE_downstream f2 n I)) = filesystem (CREATE_downstream f2 n (STORE_downstream f1 mo mn I))"
-  using O1pre O2pre
-  unfolding STORE_downstream_def CREATE_downstream_def CREATE_atSource_def STORE_atSource_def
-  by (smt case_prodE fun_upd_other fun_upd_twist option.case_eq_if snd_conv)
-
-  thus ?thesis
-  using A1
-  by (simp add: prod.expand)
+  have A1: "folderset (store f1 mo mn (create f2 n I)) = folderset (create f2 n (store f1 mo mn I))"
+    by (simp add: create_def store_folderset)
+  have "filesystem (store f1 mo mn (create f2 n I)) = filesystem (create f2 n (store f1 mo mn I))"
+    using O1pre O2pre
+    unfolding store_def create_def create_pre_def store_pre_def lookup_def 
+    by (smt case_prodE fun_upd_other fun_upd_twist option.case_eq_if snd_conv)
+  thus ?thesis by (simp add: A1 prod.expand)
+qed
+  
+-- "Case 8"
+lemma comm_delete_store:
+fixes
+  I :: "('a, 'b) imap" and
+  f1 :: "'a" and
+  f2 :: "'a" and
+  mo :: "'b" and
+  mn :: "'b" and
+  R :: "'a orset"
+assumes
+  O1pre: "store_pre f1 mo mn I" and
+  O2pre: "delete_pre f2 R I"
+shows "store f1 mo mn (delete f2 R I) = delete f2 R (store f1 mo mn I)"
+proof -
+  have A1: "folderset (store f1 mo mn (delete f2 R I)) = folderset(delete f2 R (store f1 mo mn I))"
+    by (simp add: delete_def store_folderset)
+  have "filesystem (store f1 mo mn (delete f2 R I)) = filesystem(delete f2 R (store f1 mo mn I))"
+    using O1pre O2pre
+    unfolding store_def delete_def delete_pre_def store_pre_def
+    by (simp add: fun_upd_twist option.case_eq_if)
+  thus ?thesis by (simp add: A1 prod.expand)
+qed
+  
+-- "Case 11"
+lemma comm_append_store:
+fixes
+  I :: "('a, 'b) imap" and
+  f1 :: "'a" and
+  f2 :: "'a" and
+  mo :: "'b" and
+  mn :: "'b" and
+  m :: "'b"
+assumes
+  O1pre: " store_pre f1 mo mn I" and
+  O2pre: " append_pre f2 m I"
+shows "store f1 mo mn (append f2 m I) = append f2 m (store f1 mo mn I)"
+proof -
+  have A1: "folderset (store f1 mo mn (append f2 m I)) = folderset (append f2 m (store f1 mo mn I))"
+    by (simp add: append_def store_folderset)
+  have "filesystem (store f1 mo mn (append f2 m I)) = filesystem(append f2 m (store f1 mo mn I))"
+    using O1pre O2pre unfolding store_def append_def append_pre_def store_pre_def Msg_def msgLookup_def
+    apply (simp add: case_prod_beta') 
+    by (smt Diff_empty Diff_insert0 Un_Diff Un_insert_left Un_insert_right fun_upd_twist fun_upd_upd insert_Diff insert_Diff1 map_upd_Some_unfold option.case_eq_if option.collapse option.simps(3) singletonI snd_conv)
+  thus ?thesis using A1 by (simp add: prod.expand)
 qed
 
+-- "Case 13"
+lemma comm_store_store:
+fixes
+  I :: "('a, 'b) imap" and
+  f1 :: "'a" and
+  f2 :: "'a" and
+  mo1 :: "'b" and
+  mo2 :: "'b" and
+  mn1 :: "'b" and
+  mn2 :: "'b"
+assumes
+  O1pre: " store_pre f1 mo1 mn1 I" and
+  O2pre: " store_pre f2 mo2 mn2 I"
+shows "store f1 mo1 mn1 (store f2 mo2 mn2 I) = store f2 mo2 mn2 (store f1 mo1 mn1 I)"
+proof -
+  have A1: "folderset (store f1 mo1 mn1 (store f2 mo2 mn2 I)) = folderset(store f2 mo2 mn2 (store f1 mo1 mn1 I))"
+    by (simp add: store_folderset)
+
+  have A2: "\<forall> f . f1 \<noteq> f2 \<longrightarrow> filesystem (store f1 mo1 mn1 (store f2 mo2 mn2 I)) f = filesystem(store f2 mo2 mn2 (store f1 mo1 mn1 I)) f"
+    by (smt store_def fun_upd_twist option.case_eq_if snd_conv store_filesystem)
+
+  have "f1 = f2 \<longrightarrow> filesystem (store f1 mo1 mn1 (store f2 mo2 mn2 I)) f1 = filesystem(store f2 mo2 mn2 (store f1 mo1 mn1 I)) f1"
+  proof auto
+    assume Ass: "f1 = f2"
+
+    hence "filesystem (store f1 mo1 mn1 (store f2 mo2 mn2 I)) f1 \<noteq> None"
+      by (smt O2pre store_def fun_upd_eqD fun_upd_triv option.case_eq_if option.simps(3) snd_conv store_not_none)
+
+    hence "\<exists> y . filesystem (store f1 mo1 mn1 (store f2 mo2 mn2 I)) f1 = Some y"
+      by simp
+
+    then obtain y
+    where Ass4: "filesystem (store f1 mo1 mn1 (store f2 mo2 mn2 I)) f1 = Some y"
+      by blast
+
+    have "\<exists> S . filesystem (I) f1 = Some S"
+      by (metis O2pre store_pre_def \<open>f1 = f2\<close> case_optionE msgLookup_def)
+
+    then obtain S
+    where Ass2: "(filesystem I) f1 = Some S"
+      by blast
+
+    have "\<exists> x . filesystem (store f2 mo2 mn2 I) f1 = Some x"
+      using Ass
+      by (metis O2pre option.collapse store_not_none)
+    then obtain x where Ass3: "filesystem (store f2 mo2 mn2 I) f1 = Some x"
+      by blast
+    have "x = (S - {mo2}) \<union> {mn2}"
+      using Ass Ass2 Ass3
+      unfolding store_def Msg_def
+      by simp
+    hence Ass6: "y = (S - {mo1,mo2}) \<union> {mn1,mn2}"
+      using Ass Ass2 Ass3 Ass4 O1pre O2pre
+      unfolding store_def Msg_def store_pre_def
+      by auto
+    have "\<exists> w . filesystem (store f1 mo1 mn1 I) f1 = Some w"
+      using Ass
+      by (metis O1pre option.collapse store_not_none)
+    then obtain w where Ass8: "filesystem (store f1 mo1 mn1 I) f1 = Some w"
+      by blast
+    hence Ass9: "w = (S - {mo1}) \<union> {mn1}"
+      using Ass Ass2
+      unfolding store_def Msg_def
+      by simp
+    have "filesystem(store f2 mo2 mn2 (store f1 mo1 mn1 I)) f1 \<noteq> None"
+      using O1pre Ass Ass2
+      unfolding store_def
+      by auto
+    hence "\<exists> z . filesystem(store f2 mo2 mn2 (store f1 mo1 mn1 I)) f1 = Some z"
+      by simp
+    then obtain z where Ass7: "filesystem(store f2 mo2 mn2 (store f1 mo1 mn1 I)) f1 = Some z"
+      by blast
+    hence "z = (S - {mo1,mo2}) \<union> {mn1,mn2}"
+      using Ass Ass2 Ass9 Ass8 O1pre O2pre
+      unfolding store_def Msg_def store_pre_def
+      by auto
+    thus "filesystem (store f2 mo1 mn1 (store f2 mo2 mn2 I)) f2 = filesystem (store f2 mo2 mn2 (store f2 mo1 mn1 I)) f2"
+      using Ass7 Ass4 Ass6 Ass
+      by auto
+  qed
+
+  thus ?thesis
+  using A1 A2
+  by (smt O1pre O2pre store_def fun_upd_same fun_upd_twist fun_upd_upd option.case_eq_if prod_eqI snd_conv store_not_none)
+qed
+-- "###############################################"
+-- "### Framework ###"
+-- "###############################################"  
+
+datatype ('a, 'b) ops = Create 'a nat | Delete 'a "'a orset" | Append 'a 'b | Store 'a 'b 'b
+
+fun imap_downstream :: "('a, 'b) ops \<Rightarrow> ('a, 'b) imap \<Rightarrow> ('a,'b) imap" where
+  "imap_downstream (Create f n) imap = create f n imap"
+| "imap_downstream (Delete f R) imap = delete f R imap"
+| "imap_downstream (Append f m) imap = append f m imap"
+| "imap_downstream (Store f mo mn) imap = store f mo mn imap"
+  
+  
+fun imap_atSource :: "('a, 'b) ops \<Rightarrow> ('a, 'b) imap \<Rightarrow> bool" where
+  "imap_atSource (Create f n) imap = create_pre f n imap"
+| "imap_atSource (Delete f R) imap = delete_pre f R imap"
+| "imap_atSource (Append f m) imap = append_pre f m imap"
+| "imap_atSource (Store f mo mn) imap = store_pre f mo mn imap"
+  
+theorem imap_comm :
+fixes
+  I :: "('a, 'b) imap" and
+  O1 :: "('a, 'b) ops" and
+  O2 :: "('a, 'b) ops"
+assumes
+  O1pre: "imap_atSource O1 I" and
+  O2pre: "imap_atSource O2 I"
+shows "imap_downstream O2 (imap_downstream O1 I) = imap_downstream O1 (imap_downstream O2 I)"    
+proof (cases O1)
+  case (Create f1 n1)
+  assume C1: "O1 = Create f1 n1"
+  then show ?thesis 
+    proof (cases O2)
+      case (Create f2 n2)
+      then show ?thesis using C1 comm_create_create O1pre O2pre by simp
+    next
+      case (Delete f2 R)
+      then show ?thesis using C1 comm_create_delete O1pre O2pre by simp
+    next
+      case (Append f2 m)
+      then show ?thesis using C1 comm_create_append O1pre O2pre by simp
+    next
+      case (Store f2 mo mn)
+      then show ?thesis using C1 comm_create_store O1pre O2pre by simp
+    qed
+next
+  case (Delete f1 R1)
+  assume C2: "O1 = Delete f1 R1"
+  then show ?thesis
+    proof (cases O2)
+      case (Create f2 n)
+      then show ?thesis using C2 comm_create_delete[of f1 R1 I f2 n] O1pre O2pre by simp
+    next
+      case (Delete f2 R2)
+      then show ?thesis using C2 comm_delete_delete O1pre O2pre by simp
+    next
+      case (Append f2 m)
+      then show ?thesis using C2 comm_delete_append O1pre O2pre by simp
+    next
+      case (Store f2 mo mn)
+      then show ?thesis using C2 comm_delete_store O1pre O2pre by simp
+    qed
+next
+  case (Append f1 m1)
+  assume C3: "O1 = Append f1 m1"
+  then show ?thesis
+    proof (cases O2)
+      case (Create f2 n)
+      then show ?thesis using C3 comm_create_append[of f1 m1 I f2 n] O1pre O2pre by simp
+    next
+      case (Delete f2 R)
+      then show ?thesis using C3 comm_delete_append[of f1 m1 I f2 R] O1pre O2pre by simp
+    next
+      case (Append f2 m2)
+      then show ?thesis using C3 comm_append_append O1pre O2pre by simp
+    next
+      case (Store f2 mo mn)
+      then show ?thesis using C3 comm_append_store O1pre O2pre by simp
+    qed
+next
+  case (Store f1 mo1 mn1)
+  assume C4: "O1 = Store f1 mo1 mn1"
+  then show ?thesis
+    proof (cases O2)
+      case (Create f2 n)
+      then show ?thesis using C4 comm_create_store[of f1 mo1 mn1 I f2 n] O1pre O2pre by simp
+    next
+      case (Delete f2 R)
+      then show ?thesis using C4 comm_delete_store[of f1 mo1 mn1 I f2 R] O1pre O2pre by simp
+    next
+      case (Append f2 m2)
+      then show ?thesis using C4 comm_append_store[of f1 mo1 mn1 I f2 m2] O1pre O2pre by simp
+    next
+      case (Store f2 mo mn)
+      then show ?thesis using C4 comm_store_store O1pre O2pre by simp
+    qed
+qed
+  
+-- "###############################################"
+-- "### TODO ###"
+-- "###############################################"
 
 -- "Case 5"
 lemma commCREATE_EXPUNGE:
@@ -473,116 +738,23 @@ fixes
   n :: nat
 assumes
   O1pre: " EXPUNGE_atSource f1 m I" and
-  O2pre: " CREATE_atSource f2 I"
-shows "EXPUNGE_downstream f1 m (CREATE_downstream f2 n I) = CREATE_downstream f2 n (EXPUNGE_downstream f1 m I)"
+  O2pre: " create_pre f2 n I"
+shows "EXPUNGE_downstream f1 m (create f2 n I) = create f2 n (EXPUNGE_downstream f1 m I)"
 proof -
-  have A1: "folderset (EXPUNGE_downstream f1 m (CREATE_downstream f2 n I)) = folderset (CREATE_downstream f2 n (EXPUNGE_downstream f1 m I))"
-  unfolding CREATE_downstream_def EXPUNGE_downstream_def
+  have A1: "folderset (EXPUNGE_downstream f1 m (create f2 n I)) = folderset (create f2 n (EXPUNGE_downstream f1 m I))"
+  unfolding create_def EXPUNGE_downstream_def
   by simp
 
-  have "filesystem (EXPUNGE_downstream f1 m (CREATE_downstream f2 n I)) = filesystem (CREATE_downstream f2 n (EXPUNGE_downstream f1 m I))"
+  have "filesystem (EXPUNGE_downstream f1 m (create f2 n I)) = filesystem (create f2 n (EXPUNGE_downstream f1 m I))"
   using O1pre O2pre
-  unfolding EXPUNGE_atSource_def EXPUNGE_downstream_def CREATE_atSource_def CREATE_downstream_def
+  unfolding EXPUNGE_atSource_def EXPUNGE_downstream_def create_pre_def create_def
   by (simp add: fun_upd_twist option.case_eq_if)
 
   thus ?thesis
   using A1 prod_eqI
   by blast
 qed
-
-
--- "Case 6"
-lemma commDELETE_DELETE:
-fixes
-  I :: "('a, 'b) imap" and
-  R1 :: "'a orset" and
-  R2 :: "'a orset" and
-  e1 :: "'a" and
-  e2 :: "'a"
-assumes
-  O1R1: " R1 = DELETE_atSource e1 I" and
-  O2R2: " R2 = DELETE_atSource e2 I"
-shows "DELETE_downstream e2 R2 (DELETE_downstream e1 R1 I) = DELETE_downstream e1 R1 (DELETE_downstream e2 R2 I)"
-proof -
-  show ?thesis using O1R1 O2R2 commRemove unfolding DELETE_downstream_def DELETE_atSource_def remove_atSource_def apply simp
-  proof -
-    assume a1: "R1 = {(a, b). (a, b) \<in> folderset I \<and> a = e1}"
-    assume a2: "R2 = {(a, b). (a, b) \<in> folderset I \<and> a = e2}"
-
-    have f3: "\<forall>P a Pa Pb aa. (P \<noteq> remove_atSource (a::'a) Pa \<or> Pb \<noteq> remove_atSource aa Pa) \<or> remove_downstream Pb (remove_downstream P Pa) = remove_downstream P (remove_downstream Pb Pa)"
-    by (meson commRemove)
-
-    have f4: "{(a, n). (a, n) \<in> folderset I \<and> a = e1} = remove_atSource e1 (folderset I)"
-    using a1
-    by (simp add: DELETE_atSource_def O1R1)
-
-    have "{(a, n). (a, n) \<in> folderset I \<and> a = e2} = remove_atSource e2 (folderset I)"
-    using a2
-    by (simp add: DELETE_atSource_def O2R2)
-
-    then show "remove_downstream {(a, n). (a, n) \<in> folderset I \<and> a = e2} (remove_downstream {(a, n). (a, n) \<in> folderset I \<and> a = e1} (folderset I)) = remove_downstream {(a, n). (a, n) \<in> folderset I \<and> a = e1} (remove_downstream {(a, n). (a, n) \<in> folderset I \<and> a = e2} (folderset I)) \<and> (filesystem I)(e1 := None, e2 := None) = (filesystem I) (e2 := None, e1 := None)"
-    using f4 f3
-    by auto
-  qed
-qed
-
-
--- "Case 7"
-lemma commDELETE_APPEND:
-fixes
-  I :: "('a, 'b) imap" and
-  f :: "'a" and
-  e :: "'a" and
-  m :: "'b" and
-  R :: "'a orset"
-assumes
-  O1pre: " APPEND_atSource f m I" and
-  O2pre: " R = DELETE_atSource e I"
-shows "APPEND_downstream f m (DELETE_downstream e R I) = DELETE_downstream e R (APPEND_downstream f m I)"
-proof -
-  have A1: "folderset(APPEND_downstream f m (DELETE_downstream e R I)) = folderset(DELETE_downstream e R (APPEND_downstream f m I))"
-  unfolding DELETE_downstream_def
-  by (simp add: append_folderset)
-
-  have "filesystem(APPEND_downstream f m (DELETE_downstream e R I)) = filesystem(DELETE_downstream e R (APPEND_downstream f m I))"
-  using O1pre O2pre
-  unfolding APPEND_atSource_def APPEND_downstream_def DELETE_atSource_def DELETE_downstream_def
-  by (simp add: fun_upd_twist option.case_eq_if)
-
-  thus ?thesis
-  using A1 prod_eqI
-  by blast
-qed
-
-
--- "Case 8"
-lemma commDELETE_STORE:
-fixes
-  I :: "('a, 'b) imap" and
-  f1 :: "'a" and
-  f2 :: "'a" and
-  mo :: "'b" and
-  mn :: "'b" and
-  R :: "'a orset"
-assumes
-  O1pre: " STORE_atSource f1 mo mn I" and
-  O2pre: " R = DELETE_atSource f2 I"
-shows "STORE_downstream f1 mo mn (DELETE_downstream f2 R I) = DELETE_downstream f2 R (STORE_downstream f1 mo mn I)"
-proof -
-  have A1: "folderset (STORE_downstream f1 mo mn (DELETE_downstream f2 R I)) = folderset(DELETE_downstream f2 R (STORE_downstream f1 mo mn I))"
-  by (simp add: DELETE_downstream_def store_folderset)
-
-  have "filesystem (STORE_downstream f1 mo mn (DELETE_downstream f2 R I)) = filesystem(DELETE_downstream f2 R (STORE_downstream f1 mo mn I))"
-  using O1pre O2pre
-  unfolding STORE_downstream_def DELETE_downstream_def DELETE_atSource_def STORE_atSource_def
-  by (simp add: fun_upd_twist option.case_eq_if)
-
-  thus ?thesis
-  using A1
-  by (simp add: prod.expand)
-qed
-
-
+  
 -- "Case 9"
 lemma commDELETE_EXPUNGE:
 fixes
@@ -593,81 +765,22 @@ fixes
   R :: "'a orset"
 assumes
   O1pre: " EXPUNGE_atSource f1 m I" and
-  O2pre: " R = DELETE_atSource f2 I"
-shows "EXPUNGE_downstream f1 m (DELETE_downstream f2 R I) = DELETE_downstream f2 R (EXPUNGE_downstream f1 m I)"
+  O2pre: " delete_pre f2 R I"
+shows "EXPUNGE_downstream f1 m (delete f2 R I) = delete f2 R (EXPUNGE_downstream f1 m I)"
 proof -
-  have A1: "folderset(EXPUNGE_downstream f1 m (DELETE_downstream f2 R I)) = folderset (DELETE_downstream f2 R (EXPUNGE_downstream f1 m I))"
-  unfolding DELETE_downstream_def EXPUNGE_downstream_def
+  have A1: "folderset(EXPUNGE_downstream f1 m (delete f2 R I)) = folderset (delete f2 R (EXPUNGE_downstream f1 m I))"
+  unfolding delete_def EXPUNGE_downstream_def
   by simp
 
-  have "filesystem(EXPUNGE_downstream f1 m (DELETE_downstream f2 R I)) = filesystem (DELETE_downstream f2 R (EXPUNGE_downstream f1 m I))"
+  have "filesystem(EXPUNGE_downstream f1 m (delete f2 R I)) = filesystem (delete f2 R (EXPUNGE_downstream f1 m I))"
   using O1pre O2pre
-  unfolding EXPUNGE_atSource_def EXPUNGE_downstream_def DELETE_atSource_def DELETE_downstream_def msgLookup_def
+  unfolding EXPUNGE_atSource_def EXPUNGE_downstream_def delete_pre_def delete_def msgLookup_def
   by (simp add: fun_upd_twist option.case_eq_if)
 
   thus ?thesis
   using A1 prod_eqI
   by blast
 qed
-
-
--- "Case 10"
-lemma commAPPEND_APPEND:
-fixes
-  I :: "('a, 'b) imap" and
-  f1 :: "'a" and
-  f2 :: "'a" and
-  m1 :: "'b" and
-  m2 :: "'b"
-assumes
-  O1pre: " APPEND_atSource f1 m1 I" and
-  O2pre: " APPEND_atSource f2 m2 I" and
-  freshm: "m1 \<noteq> m2"
-shows "APPEND_downstream f1 m1 (APPEND_downstream f2 m2 I) = APPEND_downstream f2 m2 (APPEND_downstream f1 m1 I)"
-proof -
-  have A1: "folderset(APPEND_downstream f1 m1 (APPEND_downstream f2 m2 I)) = folderset(APPEND_downstream f2 m2 (APPEND_downstream f1 m1 I))"
-  by (simp add: APPEND_downstream_def)
-
-  have "filesystem(APPEND_downstream f1 m1 (APPEND_downstream f2 m2 I)) = filesystem(APPEND_downstream f2 m2 (APPEND_downstream f1 m1 I))"
-  using O1pre O2pre freshm
-  unfolding APPEND_downstream_def APPEND_atSource_def msgLookup_def
-  by (smt Un_insert_right fun_upd_twist fun_upd_upd insert_commute map_upd_Some_unfold option.case_eq_if option.collapse option.simps(3) snd_conv sup_bot.right_neutral)
-
-  thus ?thesis
-  using A1
-  by (simp add: prod_eq_iff)
-qed
-
-
--- "Case 11"
-lemma commAPPEND_STORE:
-fixes
-  I :: "('a, 'b) imap" and
-  f1 :: "'a" and
-  f2 :: "'a" and
-  mo :: "'b" and
-  mn :: "'b" and
-  m :: "'b"
-assumes
-  O1pre: " STORE_atSource f1 mo mn I" and
-  O2pre: " APPEND_atSource f2 m I" and
-  freshmn: "m \<noteq> mn" and
-  freshmo: "m \<noteq> mo"
-shows "STORE_downstream f1 mo mn (APPEND_downstream f2 m I) = APPEND_downstream f2 m (STORE_downstream f1 mo mn I)"
-proof -
-  have A1: "folderset (STORE_downstream f1 mo mn (APPEND_downstream f2 m I)) = folderset (APPEND_downstream f2 m (STORE_downstream f1 mo mn I))"
-  by (simp add: APPEND_downstream_def store_folderset)
-
-  have "filesystem (STORE_downstream f1 mo mn (APPEND_downstream f2 m I)) = filesystem(APPEND_downstream f2 m (STORE_downstream f1 mo mn I))"
-  using O1pre O2pre freshmn freshmo
-  unfolding STORE_downstream_def APPEND_downstream_def APPEND_atSource_def STORE_atSource_def replaceMsg_def
-  by (smt Diff_insert0 Un_Diff Un_Diff_cancel2 Un_insert_right empty_iff fun_upd_twist fun_upd_upd insert_iff insert_is_Un map_upd_Some_unfold option.case_eq_if option.collapse option.simps(5) snd_conv sup_bot.right_neutral)
-
-  thus ?thesis
-  using A1
-  by (simp add: prod.expand)
-qed
-
 
 -- "Case 12"
 lemma commAPPEND_EXPUNGE:
@@ -679,125 +792,22 @@ fixes
   m2 :: "'b"
 assumes
   O1pre: "EXPUNGE_atSource f1 m1 I" and
-  O2pre: "APPEND_atSource f2 m2 I"
-shows "EXPUNGE_downstream f1 m1 (APPEND_downstream f2 m2 I) = APPEND_downstream f2 m2 (EXPUNGE_downstream f1 m1 I)"
+  O2pre: "append_pre f2 m2 I"
+shows "EXPUNGE_downstream f1 m1 (append f2 m2 I) = append f2 m2 (EXPUNGE_downstream f1 m1 I)"
 proof -
-  have A1: "folderset (EXPUNGE_downstream f1 m1 (APPEND_downstream f2 m2 I)) = folderset (APPEND_downstream f2 m2 (EXPUNGE_downstream f1 m1 I))"
-  unfolding EXPUNGE_downstream_def APPEND_downstream_def
+  have A1: "folderset (EXPUNGE_downstream f1 m1 (append f2 m2 I)) = folderset (append f2 m2 (EXPUNGE_downstream f1 m1 I))"
+  unfolding EXPUNGE_downstream_def append_def
   by simp
 
-  have "filesystem (EXPUNGE_downstream f1 m1 (APPEND_downstream f2 m2 I)) = filesystem (APPEND_downstream f2 m2 (EXPUNGE_downstream f1 m1 I))"
+  have "filesystem (EXPUNGE_downstream f1 m1 (append f2 m2 I)) = filesystem (append f2 m2 (EXPUNGE_downstream f1 m1 I))"
   using O1pre O2pre
-  unfolding EXPUNGE_downstream_def EXPUNGE_atSource_def APPEND_downstream_def APPEND_atSource_def
+  unfolding EXPUNGE_downstream_def EXPUNGE_atSource_def append_def append_pre_def
   by (smt Diff_empty Diff_insert0 Un_Diff case_prod_beta' fun_upd_apply fun_upd_twist fun_upd_upd insert_Diff insert_Diff1 map_upd_eqD1 mk_disjoint_insert msgLookup_def option.case_eq_if option.collapse option.simps(3) singletonI snd_conv)
 
   thus ?thesis
   using A1 prod_eqI
   by blast
 qed
-
-
--- "Case 13"
-lemma commSTORE_STORE:
-fixes
-  I :: "('a, 'b) imap" and
-  f1 :: "'a" and
-  f2 :: "'a" and
-  mo1 :: "'b" and
-  mo2 :: "'b" and
-  mn1 :: "'b" and
-  mn2 :: "'b"
-assumes
-  O1pre: " STORE_atSource f1 mo1 mn1 I" and
-  O2pre: " STORE_atSource f2 mo2 mn2 I"
-shows "STORE_downstream f1 mo1 mn1 (STORE_downstream f2 mo2 mn2 I) = STORE_downstream f2 mo2 mn2 (STORE_downstream f1 mo1 mn1 I)"
-proof -
-  have A1: "folderset (STORE_downstream f1 mo1 mn1 (STORE_downstream f2 mo2 mn2 I)) = folderset(STORE_downstream f2 mo2 mn2 (STORE_downstream f1 mo1 mn1 I))"
-  by (simp add: store_folderset)
-
-  have A2: "\<forall> f . f1 \<noteq> f2 \<longrightarrow> filesystem (STORE_downstream f1 mo1 mn1 (STORE_downstream f2 mo2 mn2 I)) f = filesystem(STORE_downstream f2 mo2 mn2 (STORE_downstream f1 mo1 mn1 I)) f"
-  by (smt STORE_downstream_def fun_upd_twist option.case_eq_if snd_conv store_filesystem)
-
-  have "f1 = f2 \<longrightarrow> filesystem (STORE_downstream f1 mo1 mn1 (STORE_downstream f2 mo2 mn2 I)) f1 = filesystem(STORE_downstream f2 mo2 mn2 (STORE_downstream f1 mo1 mn1 I)) f1"
-  proof auto
-    assume Ass: "f1 = f2"
-
-    hence "filesystem (STORE_downstream f1 mo1 mn1 (STORE_downstream f2 mo2 mn2 I)) f1 \<noteq> None"
-    by (smt O2pre STORE_downstream_def fun_upd_eqD fun_upd_triv option.case_eq_if option.simps(3) snd_conv store_not_none)
-
-    hence "\<exists> y . filesystem (STORE_downstream f1 mo1 mn1 (STORE_downstream f2 mo2 mn2 I)) f1 = Some y"
-    by simp
-
-    then obtain y
-    where Ass4: "filesystem (STORE_downstream f1 mo1 mn1 (STORE_downstream f2 mo2 mn2 I)) f1 = Some y"
-    by blast
-
-    have "\<exists> S . filesystem (I) f1 = Some S"
-    by (metis O2pre STORE_atSource_def \<open>f1 = f2\<close> case_optionE msgLookup_def)
-
-    then obtain S
-    where Ass2: "(filesystem I) f1 = Some S"
-    by blast
-
-    have "\<exists> x . filesystem (STORE_downstream f2 mo2 mn2 I) f1 = Some x"
-    using Ass
-    by (metis O2pre option.collapse store_not_none)
-
-    then obtain x
-    where Ass3: "filesystem (STORE_downstream f2 mo2 mn2 I) f1 = Some x"
-    by blast
-
-    have "x = (S - {mo2}) \<union> {mn2}"
-    using Ass Ass2 Ass3
-    unfolding STORE_downstream_def replaceMsg_def
-    by simp
-
-    hence Ass6: "y = (S - {mo1,mo2}) \<union> {mn1,mn2}"
-    using Ass Ass2 Ass3 Ass4 O1pre O2pre
-    unfolding STORE_downstream_def replaceMsg_def STORE_atSource_def
-    by auto
-
-    have "\<exists> w . filesystem (STORE_downstream f1 mo1 mn1 I) f1 = Some w"
-    using Ass
-    by (metis O1pre option.collapse store_not_none)
-
-    then obtain w
-    where Ass8: "filesystem (STORE_downstream f1 mo1 mn1 I) f1 = Some w"
-    by blast
-
-    hence Ass9: "w = (S - {mo1}) \<union> {mn1}"
-    using Ass Ass2
-    unfolding STORE_downstream_def replaceMsg_def
-    by simp
-
-    have "filesystem(STORE_downstream f2 mo2 mn2 (STORE_downstream f1 mo1 mn1 I)) f1 \<noteq> None"
-    using O1pre
-    unfolding STORE_downstream_def
-    using Ass Ass2
-    by auto
-
-    hence "\<exists> z . filesystem(STORE_downstream f2 mo2 mn2 (STORE_downstream f1 mo1 mn1 I)) f1 = Some z"
-    by simp
-
-    then obtain z
-    where Ass7: "filesystem(STORE_downstream f2 mo2 mn2 (STORE_downstream f1 mo1 mn1 I)) f1 = Some z"
-    by blast
-
-    hence "z = (S - {mo1,mo2}) \<union> {mn1,mn2}"
-    using Ass Ass2 Ass9 Ass8 O1pre O2pre
-    unfolding STORE_downstream_def replaceMsg_def STORE_atSource_def
-    by auto
-
-    thus "filesystem (STORE_downstream f2 mo1 mn1 (STORE_downstream f2 mo2 mn2 I)) f2 = filesystem (STORE_downstream f2 mo2 mn2 (STORE_downstream f2 mo1 mn1 I)) f2"
-    using Ass7 Ass4 Ass6 Ass
-    by auto
-  qed
-
-  thus ?thesis
-  using A1 A2
-  by (smt O1pre O2pre STORE_downstream_def fun_upd_same fun_upd_twist fun_upd_upd option.case_eq_if prod_eqI snd_conv store_not_none)
-qed
-
 
 -- "Case 14"
 lemma commSTORE_EXPUNGE:
@@ -810,31 +820,31 @@ fixes
   mn :: "'b"
 assumes
   O1pre: "EXPUNGE_atSource f1 m1 I" and
-  O2pre: "STORE_atSource f2 mo mn I"
-shows "EXPUNGE_downstream f1 m1 (STORE_downstream f2 mo mn I) = STORE_downstream f2 mo mn (EXPUNGE_downstream f1 m1 I)"
+  O2pre: "store_pre f2 mo mn I"
+shows "EXPUNGE_downstream f1 m1 (store f2 mo mn I) = store f2 mo mn (EXPUNGE_downstream f1 m1 I)"
 proof -
-  have A1: "folderset (EXPUNGE_downstream f1 m1 (STORE_downstream f2 mo mn I)) = folderset (STORE_downstream f2 mo mn (EXPUNGE_downstream f1 m1 I))"
-  unfolding EXPUNGE_downstream_def STORE_downstream_def
+  have A1: "folderset (EXPUNGE_downstream f1 m1 (store f2 mo mn I)) = folderset (store f2 mo mn (EXPUNGE_downstream f1 m1 I))"
+  unfolding EXPUNGE_downstream_def store_def
   by simp
 
-  have A2: "\<forall> f . f1 \<noteq> f2 \<longrightarrow> filesystem (EXPUNGE_downstream f1 m1 (STORE_downstream f2 mo mn I)) f = filesystem (STORE_downstream f2 mo mn (EXPUNGE_downstream f1 m1 I)) f"
+  have A2: "\<forall> f . f1 \<noteq> f2 \<longrightarrow> filesystem (EXPUNGE_downstream f1 m1 (store f2 mo mn I)) f = filesystem (store f2 mo mn (EXPUNGE_downstream f1 m1 I)) f"
   using O1pre O2pre
-  unfolding EXPUNGE_downstream_def EXPUNGE_atSource_def STORE_downstream_def STORE_atSource_def
+  unfolding EXPUNGE_downstream_def EXPUNGE_atSource_def store_def store_pre_def
   by (smt fun_upd_other fun_upd_twist option.case_eq_if snd_conv)
 
-  have A3: "\<forall> f . (f1 = f2 \<and> f \<noteq> f1) \<longrightarrow> filesystem (EXPUNGE_downstream f1 m1 (STORE_downstream f2 mo mn I)) f = filesystem (STORE_downstream f2 mo mn (EXPUNGE_downstream f1 m1 I)) f"
+  have A3: "\<forall> f . (f1 = f2 \<and> f \<noteq> f1) \<longrightarrow> filesystem (EXPUNGE_downstream f1 m1 (store f2 mo mn I)) f = filesystem (store f2 mo mn (EXPUNGE_downstream f1 m1 I)) f"
   using O1pre O2pre
-  unfolding EXPUNGE_downstream_def EXPUNGE_atSource_def STORE_downstream_def STORE_atSource_def
+  unfolding EXPUNGE_downstream_def EXPUNGE_atSource_def store_def store_pre_def
   by (smt fun_upd_other fun_upd_twist option.case_eq_if snd_conv)
 
-  have "f1 = f2 \<longrightarrow> filesystem (EXPUNGE_downstream f1 m1 (STORE_downstream f2 mo mn I)) f1 = filesystem (STORE_downstream f2 mo mn (EXPUNGE_downstream f1 m1 I)) f1"
+  have "f1 = f2 \<longrightarrow> filesystem (EXPUNGE_downstream f1 m1 (store f2 mo mn I)) f1 = filesystem (store f2 mo mn (EXPUNGE_downstream f1 m1 I)) f1"
   using O1pre O2pre
-  unfolding EXPUNGE_downstream_def EXPUNGE_atSource_def STORE_downstream_def STORE_atSource_def msgLookup_def replaceMsg_def
+  unfolding EXPUNGE_downstream_def EXPUNGE_atSource_def store_def store_pre_def msgLookup_def Msg_def
   by (smt Diff_empty Diff_insert Diff_insert0 Un_Diff empty_iff fun_upd_same insertE insert_commute map_upd_eqD1 option.case_eq_if option.collapse option.simps(3) snd_conv)
 
-  hence "filesystem (EXPUNGE_downstream f1 m1 (STORE_downstream f2 mo mn I)) = filesystem (STORE_downstream f2 mo mn (EXPUNGE_downstream f1 m1 I))"
+  hence "filesystem (EXPUNGE_downstream f1 m1 (store f2 mo mn I)) = filesystem (store f2 mo mn (EXPUNGE_downstream f1 m1 I))"
   using O1pre O2pre A2 A3
-  unfolding EXPUNGE_downstream_def EXPUNGE_atSource_def STORE_downstream_def STORE_atSource_def
+  unfolding EXPUNGE_downstream_def EXPUNGE_atSource_def store_def store_pre_def
   by fastforce
 
   thus ?thesis
