Isabelle/ORSet.thy
@@ -5,102 +5,97 @@ begin
 
 
 
--- "#############################"
--- "### Definitions & Helpers ###"
--- "#############################"
+-- "############################"
+-- "##### CRDT Definitions #####"
+-- "############################"
 
 
 type_synonym 'a orset = "('a \<times> nat) set"
-
 
 definition abstractState ::
   "'a orset \<Rightarrow> 'a set"
 where
   "abstractState S = {e . (\<exists> n . (e, n) \<in> S)}"
 
-
-definition fresh ::
-  "nat \<Rightarrow> 'a orset \<Rightarrow> bool"
-where
-  "fresh n S = (\<nexists> e . (e, n) \<in> S)"
-
-
 definition lookup ::
   "'a \<Rightarrow> 'a orset \<Rightarrow> bool"
 where
   "lookup e S = (\<exists> n. (e, n) \<in> S)"
 
-
+definition add_pre ::
+  "nat \<Rightarrow> 'element orset \<Rightarrow> bool"
+where
+  "add_pre n S = (\<nexists> e . (e, n) \<in> S)"
+  
 definition add ::
   "'element \<Rightarrow> nat \<Rightarrow> 'element orset \<Rightarrow> 'element orset"
 where
-  "add e alpha S = S \<union> {(e, alpha)}"
+  "add e n S = S \<union> {(e, n)}"
 
-
-definition remove_atSource ::
-  "'element \<Rightarrow> 'element orset \<Rightarrow> 'element orset"
+definition remove_pre ::
+  "'element \<Rightarrow> 'element orset \<Rightarrow> 'element orset \<Rightarrow> bool"
 where
-  "remove_atSource e S = {(a, b) \<in> S. a = e}"
+  "remove_pre e R S = (lookup e S \<and> (R = {(a, b) \<in> S. a = e}))"
 
-definition remove_downstream ::
+definition remove ::
   "'element orset \<Rightarrow> 'element orset \<Rightarrow> 'element orset"
 where
-  "remove_downstream R S = S - R"
+  "remove R S = S - R"
+  
+-- "#################"
+-- "### Framework ###"
+-- "#################"  
 
+datatype 'a ops = Add 'a nat | Remove 'a "'a orset"
+  
+fun orset_downstream :: "'a ops \<Rightarrow> 'a orset \<Rightarrow> 'a orset" where
+  "orset_downstream (Add e n) pl = add e n pl"
+| "orset_downstream (Remove e R) pl = remove R pl"
+  
+fun orset_atSource :: "'a ops \<Rightarrow> 'a orset \<Rightarrow> bool" where
+  "orset_atSource (Add e n) pl = add_pre n pl"
+| "orset_atSource (Remove e R) pl = remove_pre e R pl"
 
-
--- "#################################################"
--- "### Commutativity Proofs of OR-Set Operations ###"
--- "#################################################"
-
-
-lemma commAdd:
-  shows "\<forall> S . n1 \<noteq> n2 \<longrightarrow> add e1 n1 (add e2 n2 S) = add e2 n2 (add e1 n1 S)"
-proof clarify
-  fix S
-  assume "n1 \<noteq> n2"
-  then show "add e1 n1 (add e2 n2 S) = add e2 n2 (add e1 n1 S)"
-  by (simp add: Un_commute add_def)
-qed
-
-
-lemma commRemove:
+theorem orset_comm :
 fixes
   S :: "'a orset" and
-  R1 :: "'a orset" and
-  R2 :: "'a orset" and
-  e1 :: "'a" and
-  e2 :: "'a"
+  O1 :: "'a ops" and
+  O2 :: "'a ops"
 assumes
-  O1R1: " R1 = remove_atSource e1 S" and
-  O2R2: " R2 = remove_atSource e2 S"
-shows "remove_downstream R2 (remove_downstream R1 S) = remove_downstream R1 (remove_downstream R2 S)"
-proof -
-  show ?thesis
-  using O1R1 O2R2
-  unfolding remove_atSource_def remove_downstream_def
-  by auto
+  O1pre: "orset_atSource O1 S" and
+  O2pre: "orset_atSource O2 S"
+shows "orset_downstream O2 (orset_downstream O1 S) = orset_downstream O1 (orset_downstream O2 S)"    
+proof (cases O1)  
+  case (Add e1 n1)
+  assume C1: "O1 = Add e1 n1"
+  then show ?thesis 
+    proof (cases O2)
+      case (Add e2 n2)
+      then show ?thesis
+      using C1 O1pre O2pre
+      by (simp add: Un_commute add_def)
+    next
+      case (Remove e2 R)
+      then show ?thesis
+      using C1 O1pre O2pre
+      apply (simp add: add_pre_def add_def remove_pre_def remove_def) 
+      by auto
+    qed
+next
+  case (Remove e1 R1)
+  assume C2: "O1 = Remove e1 R1"
+  then show ?thesis 
+    proof (cases O2)
+      case (Add e2 n)
+      then show ?thesis using C2 O1pre O2pre
+      apply (simp add: add_pre_def add_def remove_pre_def remove_def)
+      by auto        
+    next
+      case (Remove e2 R)
+      then show ?thesis using C2 O1pre O2pre
+      apply (simp add: remove_def remove_pre_def) 
+      by auto
+    qed
 qed
-
-
-lemma commAddRemove:
-fixes
-  S :: "'a orset" and
-  R :: "'a orset" and
-  e1 :: "'a" and
-  e2 :: "'a" and
-  n :: nat
-assumes
-  OR: " R = remove_atSource e1 S" and
-  freshn: "fresh n S"
-shows "abstractState (remove_downstream R (add e2 n S)) = abstractState (add e2 n (remove_downstream R S))"
-proof -
-  show ?thesis
-  using OR freshn
-  unfolding abstractState_def remove_downstream_def remove_atSource_def add_def fresh_def
-  by auto
-qed
-
-
 
 end
